
\chapter{Integration}
\section{Simple Functions}

\begin{definition}
  nonnegative simple function are measurable function with finitely many values in $\RR$ (NOT on $\bar{\RR}$).
  $s: X \to \RR$, $s(x) = \sum z_j \mathbbm{1}_{x, s(z) = z_j}(x) = \sum z_j \mathbbm{1}_{f^{-1}({z_j})}$
  If values of $s$ are $\{z_1, \dotsc, z_n\}$
\end{definition}

% \pagebreak
% \begin{proof}
%   for any $v \in (\mathrm{span}(S_1) + \mathrm{span}(S_2))$, there exists $w_1 \in \mathrm{span}(S_1)$, $w_2 \in \mathrm{span}(S_2)$ such that
%   $v = w_1 + w_2$. Then, from the definiton of the span, there exists $\alpha_1, \alpha_2, \dotsc, \alpha_n \in \mathbb{F}$ and $a_1, a_2, \dotsc, a_n \in S_1$ such that 
%   \[w_1 = \sum_{i = 1}^n \alpha_ia_i\]
%   Similarly, there exists $\beta_1, \beta_2, \dotsc, \beta_m \in \mathbb{F}$ and $b_1, b_2, \dotsc, b_m \in S_2$ such that
%   \[ w_2 = \sum_{j = 1}^m \beta_jb_j\]
%   Then, since for all $a_i$, $a_i \in S_1 \cup S_2$ and for all $b_j$, $b_j \in S_1 \cup S_2$, then
%   \[v = w_1 + w_2 = \sum_{i = 1}^n \alpha_ia_i + \sum_{j = 1}^m \beta_jb_j \in \mathrm{span}(S_1 \cup S_2)\]
% \end{proof}

\begin{theorem}
  Consider nonnegative measurable function $f$.
  There exist a sequence of simple function $s_n$ such that 
  \begin{itemize}
    \item $0 \le s_n \le s_{n+1} \le f$ (i.e, $s_n(x) \le s_{n+1}(x)$)
    \item $\lim\limits_{n\to\infty}s_n(x) = f(x)$ for all $x$
    \item The convergence is uniform on all sets where $f$ is bounded.
    If $E$ is such that $|f(x)| \le M$ for all $x \in E$ then
    \[\sup_{x \in E} f(x) - s_n(x) \to 0\]
  \end{itemize}
\end{theorem}

\begin{proof}
  $s_n$ is defined so that if takes value in $[0, 2^n)$. Consider the segment $\frac{k}{2^n}$ on y-axis,
  then $$s_n(x) = \begin{cases}
    k\cdot2^{-n} & \text{if } k2^{-n} \le f(x) < (k+1)2^{-n}, 0 \le k \le 4^n - 1 \\
    2^n & \text{if } f(x) \ge 2^n
  \end{cases}$$

If $f(x) < 2^n$ then $0 \le f(x) - s_n(x) \le 2^{-n}$. We can see that $s_n(x) \le s_{n+1}(x)$ because
each step of $s_{n+1}$ is a refinement of $s_n$.
\end{proof}

We first define the integral for simple function (in analogy to the definition of Riemann-integral for stop functions)
\begin{definition}
  Define 
  $s(x) = \sum_j c_j \mathbbm{1}_{E_j}$
  where the $E_j$ are pairwise disjoint, $\biguplus E_j = X$, then
  \[\int s \ \mathrm{d}\mu = \sum_j c_j \mu(E_j)\]
\end{definition}

\begin{claim}
  $$s(x) = \sum_{j=1}^n c_j\mathbbm{1}_{E_j}(x) = \sum_{k = 1}^m d_k \mathbbm{1}_{E_k}(x)$$
  where $X = \biguplus E_j = \biguplus E_k$. If $x \in E_j \cap E_k$ then $c_j = d_k$.
\end{claim}

\begin{proof}
  We know that $\biguplus_{j, k} E_j \cap E_k = X$ and $E_j = \biguplus_{k} E_j \cap E_k$

  GOAL: $\sum_{j=1}^n c_j\mu(E_j) = \sum_{k=1}^m d_k \mu(F_k)$

  \begin{align*}
    \text{LHS}=\sum_{j=1}^n c_j \sum_{k=1}^\infty \mu(E_j \cap F_k) &= \sum_{k=1}^m \sum_{j=1}^n d_k \mu(E_j \cap E_k) \\
    &= \sum_{k=1}^m d_k \mu(F_k)
  \end{align*}
\end{proof}


\begin{lemma}
  Suppose $s, t$ are simple functions then
  \[\int (s + t)\ \mathrm{d}\mu = \int s \ \mathrm{d}\mu+ \int t\ \mathrm{d}\mu\] 
\end{lemma}

\begin{remark}
  Can shortly write 
  \[\int s + t = \int s + \int t\]
\end{remark}

\begin{proof}
  \begin{align*}
  s = \sum_{j=1}^n c_j \mathbbm{1}_{E_j} &= \sum_{j}\sum_k c_j \mathbbm{1}_{E_{j} \cap F_k} \\
  t = \sum_{k=1}^m d_k \mathbbm{1}_{F_k} &= \sum_{j}\sum_k d_k \mathbbm{1}_{E_{j} \cap F_k} \\
  s + t&= \sum_{j, k} (c_j + d_k) \mathbbm{1}_{E_j \cap F_k} \\
  \end{align*} 
  \begin{align*}
    \int s\ \mathrm{d}\mu &= \sum_{j, k}c_j \mu(E_j \cap F_k) \\
    \int t\ \mathrm{d}\mu &= \sum_{j, k}d_k \mu(E_j \cap F_k) \\
    \int (s + t)\ \mathrm{d}\mu &= \sum_{j, k}(c_j + d_k) \mu(E_j \cap F_k) \\
  \end{align*}
\end{proof}

\begin{lemma}\label{lem:measure-from-set}
  $\nu(E) = \int_E s \ \mathrm{d}\mu = \int s \mathbbm{1}_E\ \mathrm{d}\mu = \sum c_j \mu(E_j \cap E)$
  this defines a measure on $\SM$ (given $\sigma$-algebra)
\end{lemma}

\begin{proof}
  If $E^l$ is a sequence of pairwise disjoint measureable set, check
  \[\nu\left(\biguplus E^l\right) = \sum \nu(E^l)\] 
  \begin{align*}
    \nu\left(\biguplus E^l\right) &= \sum c_j \mu(E_j \cap \biguplus E^l) \\
    &= \sum_{j=1}^n c_j \sum_l \mu(E_j \cap E^l) \\
    &= \sum_l \sum_j c_j \mu(E_j \cap E^l) \\
    &= \sum_l \nu(E^l)
  \end{align*}
\end{proof}

\section{Non-negative Measurable Functions}

\begin{definition}
  For any non-negative $f$, a measurable function, define
  \[\int f \ \mathrm{d}\mu = \sup_{s \le f, s \text{ simple}} \int s \ \mathrm{d}\mu\]
\end{definition}

\begin{remark}
  If $0 \le f \leq g$ then $\int f \ \mathrm{d}\mu \leq \int g \ \mathrm{d}\mu$
\end{remark}

\begin{theorem}[Monotone Convergence Theorem]
  If $\{f_n\}$ is a sequence of measurable function, and $0 \le f_n \le f_{n+1}$ for all $n$. 
  (that means $f(x) = \lim\limits_{n\to\infty}f_n(x)$)Then
  \[\int f\ \mathrm{d}\mu = \lim_{n\to\infty}\int f_n\ \mathrm{d}\mu\]
\end{theorem}

\begin{proof}

  Since $f_n \le f_{n+1} \le f$ then 
  \begin{align*}
    \lim_{n\to\infty}\int f_n\ \mathrm{d}\mu \le \int f\ \mathrm{d}\mu
  \end{align*}
  % $\int f_n \le \int f \implies \lim_{n\to\infty} \int f_n \le \int f$.

  We need to show that $$\int f \ \mathrm{d}\mu\le \lim\limits_{n\to\infty} \int f_n\ \mathrm{d}\mu$$
  So, it suffices to show that for any $0 \le \underset{\text{simple}}s \le f$, that 

  $$\int s\ \mathrm{d}\mu \le \lim\limits_{n\to\infty} \int f_n\ \mathrm{d}\mu$$

  It suffices to show that for any $\eps > 0$, 
  $$(1-\eps)\int s\ \mathrm{d}\mu \le \lim_{n\to\infty} \int f_n\ \mathrm{d}\mu$$
  Define $E_n = \{x : (1 - \eps)s(x) \le f_n(x)\}$, any $x$ will be in one of the $E_n$.
  Then for any $x \in E_n$, 
  $$s(x) \le \frac{f_n(x)}{1-\eps}$$
  % $$(1-\eps) s(x)< \lim_{n \to \infty} f_n(x) = f(x)$$
  % This mean $(1-\eps)s(x) < f_n(x)$ for sufficiently large $n$ ($n \ge N(x)$).
  % We will show that $$\bigcup_{n=1}^\infty E_n = X$$
  Consider the measure defined by $$\nu(E) = \int_E s\ \mathrm{d}\mu$$ (we already show this is a measure in \ref{lem:measure-from-set}).
  We have $E_n \subseteq E_{n+1}$ and $E_n \to X$. By continuity from below~\ref{lem:continuity-from-below}, 
  $$\lim\limits_{n\to\infty}\nu(E_n) = \nu(X) = \int s\ \mathrm{d}\mu$$
  We get that
  $$\nu(E_n) = \int_{E_n} s\ \mathrm{d}\mu \le \int_{E_n} \frac{f_n(x)}{1-\eps}\ \mathrm{d}\mu \leq \int\frac{f_n(x)}{1-\eps}\ \mathrm{d}\mu = \frac1{1-\eps}\int f_n(x)\ \mathrm{d}\mu$$
  Finally, we take limit on both sides and we have 
  $$\lim_{n\to\infty}\nu(E_n) = \nu(\RR) = \int s\ \mathrm{d}\mu \le \lim_{n\to\infty} \frac1{1-\eps} \int f_n\ \mathrm{d}\mu$$
\end{proof}

\begin{lemma}
  If $f, g$ are non negative measurable function then 
  \[\int (f+g)\ \mathrm{d}\mu = \int f\ \mathrm{d}\mu + \int g\ \mathrm{d}\mu\]
\end{lemma}

\begin{proof}
  Now we have a tool \begin{itemize}
    \item Monotone Convergence Theorem
    \item Existence of $s_n\gg f, t_n \gg g$
  \end{itemize}
  \begin{align*}
    \int (s_n + t_n)\ \mathrm{d}\mu &= \int s_n\ \mathrm{d}\mu + \int t_n\ \mathrm{d}\mu \\
    \int (f + g)\ \mathrm{d}\mu &= \int f\ \mathrm{d}\mu + \int g\ \mathrm{d}\mu
  \end{align*}
\end{proof}

\begin{lemma}
$f_k \ge 0$, $f_k$ is measurable
$$\int \sum_{k=1}^\infty f_k(x)\ \mathrm{d}\mu = \sum_{k=1}^\infty\int f_k \ \mathrm{d}\mu$$
\end{lemma}

\begin{proof}
  Just apply the Monotone Convergence Theorem.
  \[s_n(x) = \sum_{k=1}^n f_k(x) \to \sum_{k=1}^\infty f_k(x)\]
\end{proof}

\begin{remark}
We cannot always interchange integrals and limits (monotonicity is key)
$f_n(x) = \frac1n\mathbbm{1}_{[0, n]}, \int f_n\ \mathrm{d}\mu = 1$ 
but $\lim\limits_{n\to\infty}f_n(x) = 0$.
\[0 = \int \lim_{n\to \infty} f_n(x)\ \mathrm{d}\mu < \lim_{n\to\infty}\int f_n\ \mathrm{d}\mu\]

Or on $[0, 1]$, $f_n(x) = n\mathbbm{1}_{[0, 1/n]}$, $\int f_n\ \mathrm{d}\mu = 1$ but $\lim\limits_{n\to\infty}f_n(x) = 0$. 
$$\lim\limits_{n\to\infty}f_n(x) = \begin{cases}
  \infty & \text{if } x = 0 \\ 
  0 & \text{if } x > 0
\end{cases}$$
\end{remark}
  
\begin{lemma}[Faton's Lemma]
  If $\{f_j\}$ is a sequnce of measurable functions
  \[\int\liminf_{j\to\infty}f_j(x)\ \mathrm{d}\mu \le \liminf_{j\to\infty}\int f_j \ \mathrm{d}\mu\] 
  meaning 
  \[\int\lim_{k\to\infty} \underbrace{\inf_{j\ge k}f_j(x)\ \mathrm{d}\mu}_{\text{increasing on }k} \le \lim_{k\to\infty}\inf_{j\ge k}\int f_j \ \mathrm{d}\mu\] 
\end{lemma}
\begin{proof}
  \[\int\lim_{k\to\infty} \inf_{j\ge k}f_j(x)\ \mathrm{d}\mu \underset{\text{MCT}}= \lim_{k \to \infty} \int \inf_{j \ge k}f_j(x) \ \mathrm{d}\mu \]
  Take any $l \ge k$, then $\inf_{j \ge k}f_j(x) \le f_l(x)$, then for $l \ge k$
  \begin{align*}
    \int\inf_{j\ge k}f_j(x)\ \mathrm{d}\mu &\le \int f_l(x)\ \mathrm{d}\mu \\
    \int \inf_{j\ge k}f_j(x)\ \mathrm{d}\mu &\le \inf_{j\ge k}\int f_j(x)\ \mathrm{d}\mu
  \end{align*}
\end{proof}

\section{General Measurable Functions}

Integral for ``general'' measurable functions.

\begin{definition}
  Given a measurable function $f$, we define the \textbf{positive part} of $f$ as 
  \[f^+(x) = \max\{f(x), 0\}\]
  and the \textbf{negative part} of $f$ as
  \[f^-(x) = \max\{-f(x), 0\}\]
  Then we get that 
  \[f = f^+ - f^-\]
\end{definition}

\begin{definition}
  $f: X \to \RR$ (or $\bar{\RR}$)
  Suppose that $f$ is a measurable function, then we define
  \[\int f \ \mathrm{d}\mu = \int f^+\ \mathrm{d}\mu - \int f^-\ \mathrm{d}\mu\]
  provided that at least one of $\int f^\pm \ \mathrm{d}\mu$ is finite
\end{definition}
\begin{definition}
  $f: X \to \RR$ (or $\bar{\RR}$)
  $f$ is \textbf{integrable} if $\int f^+ \ \mathrm{d}\mu$, $\int f^- \ \mathrm{d}\mu$ is finite
  $\iff$ $\int |f| \ \mathrm{d}\mu$ is finite

  $\mathcal{L}^1$ is the class of integrable function
\end{definition}

\begin{definition}
$f: X \to \CC$ is measureable ($\iff$ $\Re(f)$ and $\Im(f)$ are measurable)
Assumeing that $\Re f \in \mathcal{L}^1$ and $\Im f \in \mathcal{L}^1$ then
\[\int f\ \mathrm{d}\mu = \int \Re f \ \mathrm{d}\mu + i \int \Im f \ \mathrm{d}\mu\]
\end{definition}

\begin{claim}
  Suppose that $f, g$ are measurable then
  \[\int f + g\ \mathrm{d}\mu  = \int f\ \mathrm{d}\mu + \int g\ \mathrm{d}\mu\]
  \[\int \alpha f \ \mathrm{d}\mu + \alpha \int f \ \mathrm{d}\mu\]
\end{claim}

\begin{lemma}
  $f: X \to \bar{\RR}$ is measurable, and $\int |f| \ \mathrm{d}\mu = 0$ then $f = 0$ almost everywhere.
\end{lemma}

\begin{proof}
  Assume that $\int |f| \ \mathrm{d}\mu = 0$ Find simple function $s_n$ of $f$ then 
  $\int s_n \ \mathrm{d}\mu = 0 \implies$ $s_n(x) = 0$ almost everywhere.
  we claim that $s_n\to f$ everywhere then $s_n = 0$ almost everywhere then $f = 0$ alomost everywhere.
  There is a set $N_n, \mu(N_n) = 0$ so that $s_n = 0$ in $N_n^\complement$. 
  $N = \bigcup_{n=1}^\infty N_n \implies \mu(N) = 0$ and $N^\complement$ we have $s_n \to f$, $s_n = 0$
\end{proof}

We could redefine the notion of $f=0$ (being $f(x) = 0$ for all $x \in X$) to $f = 0$ almost everywhere (meaning $f(x) = 0$ except for all null set).


\begin{remark}
  $\|f\| = \int |f|\ \mathrm{d}\mu$ satisfies
  \begin{itemize}
    \item $\|f + g\| \le \|f\| + \|g\|$
    \item $\|c f\| = |c|\|f\|$
    \item $\|f\| = 0 \iff f = 0$ almost everywhere
  \end{itemize}
\end{remark}

\begin{remark}
  Almost everywhere equal is an equivalence relation.
  \[f \sim g \underset{\text{def}}\iff f(x) = g(x)\ \mu\text{-almost everywhere}\]
  $N = \{f \in\mathcal{L}^1 : f(x) = 0 \text{ almost everywhere}\}$ is a linear subspace of $\mathcal{L}^1$ vector.
  $\mathcal{L}^1/N$ is the set of equivalence classes of $\mathcal{L}^1$.
\end{remark}

$f_n \to f$ almose everywhere, $f_n \ge 0$, $f_n$ measurable, Can we define $\int f\ \mathrm{d}\mu$?
$f$ may not be measurable. This problem is fixed if $f$ we work in a complete measurable space
$(X, \SM, \mu) \to (X, \bar{\SM}, \bar{\mu})$
where 
\[\bar{\SM} = \{A \cup B : A \in \SM, B \text{ a subset of a set of measure }0\}\]

\begin{lemma}
$f \in \mathcal{L}^1$, $\int |f|\ \mathrm{d}\mu < \infty$. If $f$ is real valued $f = f^+ - f^-$,
\[\left|\int f\ \mathrm{d}\mu \right| \le \int |f| \ \mathrm{d}\mu\]
\end{lemma}
\begin{proof}
  \begin{align*}
    \left|\int f\ \mathrm{d}\mu \right| &= \left|\int f^+ - f^- \ \mathrm{d}\mu \right| \\
    &\le \left|\int f^+ \ \mathrm{d}\mu \right| + \left|\int f^- \ \mathrm{d}\mu \right| \\
    &= \int f^+ \ \mathrm{d}\mu + \int f^- \ \mathrm{d}\mu \\
    &= \int |f| \ \mathrm{d}\mu
  \end{align*}
\end{proof}

\begin{remark}
  If $f$ is complex valued, then $|f| = \sqrt{(\Re f)^2 + (\Im f)^2}$.
  Then
  \[\left|\int \Re f \right|\le \int |\Re f| \le \int |f|\]
  \[\left|\int \Im f \right|\le \int |\Im f| \le \int |f|\]
  So, 
  \[\left|\int f\ \mathrm{d}\mu \right| \le 2\int |f|\]
\end{remark}

\begin{remark}
  Estimate $\int f \ \mathrm{d}\mu = \alpha + i\beta = re^{i \phi}$, then
  $e^{-i\phi} \int f \ \mathrm{d}\mu$ is real and nonnegative.
  \begin{align*}
    \left|\int f \ \mathrm{d}\mu\right| &= \left|e^{-i\phi} \int f \ \mathrm{d}\mu\right| \\
    % &= \int e^{-i\phi}f \ \mathrm{d}\mu \\
    &= \Re \int e^{-i\phi}f \ \mathrm{d}\mu \\
    &\le \int |e^{-i\phi}f| \ \mathrm{d}\mu \\
    &= \int |f| \ \mathrm{d}\mu
  \end{align*}
\end{remark}

$f \in \mathcal{L}^+$ means non-negative, $\nu(E) = \int_E f \ \mathrm{d}\mu$ this is measure
Check the $\sigma$-additivity
$E = \biguplus_{n=1}^\infty E_n$, 
\begin{align*}
  \nu\left(\biguplus_{n=1}^\infty E_n\right) &= \int_{\biguplus E_n} f \ \mathrm{d}\mu \\
  &= \int f \mathbbm{1}_{\biguplus E_n} \ \mathrm{d}\mu \\
  &= \int f \left(\sum_{n=1}^\infty \mathbbm{1}_{E_n}\right) \ \mathrm{d}\mu \\
  &= \sum_{n=1}^\infty \int f \mathbbm{1}_{E_n} \ \mathrm{d}\mu \\
  &= \sum_{n=1}^\infty \nu(E_n)
\end{align*}

\begin{claim}
  If $f \in \mathcal{L}^1 \cap \mathcal{L}^+$ then $\nu$ is a finite measure.
\end{claim}

If $\nu(E) = int f  \ \mathrm{d}\mu$
How does $\int g \ \mathrm{d}\nu$ look like?
$\nu(E) = \int f \ \mathrm{d}\mu = \int E \ \mathrm{d}\nu$
We want ``$f\ \mathrm{d}\mu = \mathrm{d}\nu$''
\begin{lemma}
  If $f \in \mathcal{L}^+$ and $\nu(E) = \int_E f \ \mathrm{d}\mu$ then for any $g \in \mathcal{L}^+$ or $g \in \mathcal{L}^1$ then,   
  \[\int g\ \mathrm{d}\nu = \int g f \ \mathrm{d}\mu\]
\end{lemma}

\begin{proof}
  \begin{itemize}
    \item True for characteristic functions of measure set by the definition of $\nu$  
    \item By linearity of the integral, it is true for simple function
    \item  $s_n\nearrow g$ if $g \in \mathcal{L}^+$, by Monotone convergence theorem, 
    \[\int s_n \underset{\text{MCT}}\nearrow \int g\]
    \begin{align*}
      \int s_n \ \mathrm{d}\nu &= \int s_n f \ \mathrm{d}\mu \\
      \int g \ \mathrm{d}\nu &= \int g f \ \mathrm{d}\mu
    \end{align*}
    Then extend to general g by linearity
  \end{itemize}
\end{proof}

%TODO: break the integration chapter

\begin{theorem}
  If $X$ is a finite measure space, if $f_n$ measurable, $f_n \in \mathcal{L}^1$ (integrable) and $f_n \to f$ uniformly on $X$. 
  then $$\int |f_n - f| \ \mathrm{d}\mu \to 0$$
  and 
  $$\int f_n\ \mathrm{d}\mu \to \int f\ \mathrm{d}\mu$$
\end{theorem}
  
\begin{remark}
  Uniform convergence means
  \[\sup_{x \in X} |f_n(x) - f(x)| \to 0\]
  as $n \to \infty$
\end{remark}

\begin{proof}
  We can rewrite that term as 
  \begin{align*}
    \int |f_n - f| \ \mathrm{d}\mu &\le \int \sup_{x\in X} |f_n - f|\ \mathrm{d}\mu \\ 
    &= \mu(X) \sup_{x\in X} |f_n - f| \to 0\\
  \end{align*}
  We can rewrite $f$ as $f = (f - f_n) + (f_n)$ since $f-f_n$ converge and $f_n$ integrable so $f$ must be integrable.
  \begin{align*}
    \left|\int f_n - \int f\right| &= \left|\int (f_n - f)\ \mathrm{d}\mu\right| \\
    &\le \int |f_n - f|\ \mathrm{d}\mu 
  \end{align*}
\end{proof}

\begin{definition}
  Suppose that $f_n, f$ are measurable
  $f_n \to f$ almost uniformly if for every $\eps > 0$
  there is a measurable set $E$ such taht $\mu(E) < \eps$ and $f_n \to f$ uniformly on $E^\complement$
  ($\sup_{x\in E^\complement} |f_n(x) - f(x)| \to 0$)
\end{definition}

\begin{theorem}[Egorov's Theorem]
  If $\mu(X) < \infty$ and if $f_n \to f$ almost everywhere then 
  $f_n \to f$ almost uniformly
\end{theorem}

\begin{remark}
  $f_n(x) \to f(x)$ if for every $k$ there exists $n = n(k)$ such that
  $|f_m(x) - f(x)| < \frac1k$ for all $m \ge n(k)$
\end{remark}

\begin{proof}
  Fix $\eps > 0$, define 
  \begin{align*}
    E_n(k) &:= \left\{x : |f_m(x) - f(x)| \ge \frac1k \text{ for some }m \ge n\right\} \\
    &= \bigcup_{m \ge n} \left\{x : |f_m(x) - f(x)| \ge \frac1k\right\}
  \end{align*}
  (Given $x$ For sufficiently large $n$, $x \notin E_n(k)$), $E_n(k) \supseteq E_{n+1}(k)$
  $\bigcap_n E_n(k) = \emptyset$ because of $f_n \to f$ everywhere.
  Form the continuity from above~\ref{lem:continuity-from-above}, we get that $\lim_{n\to\infty}\mu(E_n(k)) = 0$.
  Find $n(k)$ such that $\mu(E_{n(k)}(k)) < \frac{\eps}{2^k}$, then $E = \bigcup_k E_{n(k)}(k)$ has measure $< \eps$.
  
  For $x\in \left(\bigcup_k E_{n(k)}(k)\right)^\complement = \bigcap_k E_{n(k)}(k)^\complement$
  I have for all $k$ $|f_m(x) - f(x)| < \frac1k$ for all $m \ge n(k)$.
  So, we get $f_n \to f$ uniformly on $E^\complement$.
\end{proof}